Main Adequacy complete

theories/simulations/ctxrefine/MainAdequacy.v
@@ -5,9 +5,22 @@ Require Import LSim LSimFacts MSim MSimFacts MSimCommon.
 Require Import ISim ISimFacts ClosedAdequacy TacticsInit.
 Require Import CtxRefine.
 
-Lemma inv_sandbox_event `{Σ : GRA} {X Y} x msk (ktr : _ → itree crisE Y) (e : crisE X) :
+(** This file contains the main lemma of CRIS, namely ISim.t implies ctx_refines. *)
+
+Lemma inv_sandbox_ktr `{Σ : GRA} {X Y} x msk (ktr : _ → itree crisE Y) (e : crisE X) :
   SB.sandbox msk (trigger e >>= ktr) = trigger e >>= ktr →
   SB.sandbox msk (ktr x) = ktr x.
+Proof.
+  rewrite SBRed.bind SBRed.vis; des_ifs; ss.
+  { rewrite ?bind_vis; intros H; depdes H; eapply equal_f in x; eauto.
+    revert x; rewrite SBRed.ret; ired; eauto.
+  }
+  { rewrite bind_trigger bind_vis. intros H; depdes H; ss. }
+Qed.
+
+Lemma inv_sandbox_event `{Σ : GRA} {X Y} (x: X) msk (ktr : _ → itree crisE Y) (e : crisE X) :
+  SB.sandbox msk (trigger e >>= ktr) = trigger e >>= ktr →
+  SB.sandbox msk (ktr x) = ktr x ∧ msk X e.
 Proof.
   rewrite SBRed.bind SBRed.vis; des_ifs; ss.
   { rewrite ?bind_vis; intros H; depdes H; eapply equal_f in x; eauto.
@@ -41,483 +54,18 @@ Proof.
     { rewrite SBRed.vis; des_ifs; gstep; econs; ii; ss. }
   }
 Qed.
-(* Set Implicit Arguments. *)
-
-(* AUX *)
-
-(* Lemma alist_upd_fst_in {V} a (k : key) (v : V) l
-    (IN : In a (List.map (fst ∘ fst) l)) :
-  In a (List.map (fst ∘ fst) (alist_upd k v l)).
-Proof.
-  unfold alist_upd in *.
-  induction l; ss; i; rewrite eq_rel_dec_correct; des_ifs; ss; des; eauto.
-Qed. *)
-
-(* Lemma sandbox_well_scoped
-    `{Σ : GRA} {A} (img0 img1 : bool) (msk0 msk1 : _->bool) scp0 scp1 (itr : itree crisE A)
-    (IMPL: img0 → img1)
-    (MASK : ∀ fn, msk0 fn → msk1 fn)
-    (SCP : incl scp0 scp1) :
-  SB.sandbox img1 msk1 scp1 (SB.sandbox img0 msk0 scp0 itr) = SB.sandbox img0 msk0 scp0 itr.
-Proof.
-  apply bisim_is_eq.
-  revert_until Σ. ginit. gcofix CIH. i.
-  ides itr.
-  { rewrite! SBRed.ret. gstep. econs. eauto. }
-  { rewrite! SBRed.tau. gstep. econs. gbase. eauto. }
-  rewrite <- bind_trigger. rewrite! SBRed.bind.
-  destruct e.
-  {
-    assert ((@ITree.trigger (@crisE Σ) X (inl1 a)) = trigger a) by grind.
-    rewrite H. destruct a.
-    - rewrite !SBRed.Assume !bind_trigger. des_ifs.
-      + rewrite SBRed.Assume. des_ifs.
-        * gstep. r; s. econs. i. ired. gbase; eauto.
-        * exploit IMPL; et; i; inv x0.
-      + rewrite SBRed.vis_take. des_ifs.
-        * gstep. r; s. econs. ss.
-        * gstep. r; s. econs. ss.
-    - rewrite !SBRed.AssumeRes !bind_trigger.
-      gstep. econs. i. gbase. eauto.
-    - rewrite !SBRed.Guarantee !bind_trigger.
-      gstep. econs. i. gbase. eauto.
-  }
-  destruct s; [destruct c|].
-  {
-    rewrite! SBRed.call. des_ifs; ss.
-    + rewrite SBRed.call. des_ifs.
-      * rewrite! bind_trigger.
-        gstep. econs. i. r. gbase. eauto.
-      * exfalso. rewrite (MASK fn) in Heq0; ss.
-    + rewrite /triggerUB SBRed.unwrapU.
-      ired; rewrite !bind_trigger. gstep. econs. i. ss.
-  }
-  {
-    rewrite! SBRed.spawn. des_ifs; ss.
-    + rewrite SBRed.spawn. des_ifs.
-      * rewrite! bind_trigger.
-        gstep. econs. i. r. gbase. eauto.
-      * exfalso. rewrite (MASK fn) in Heq0; ss.
-    + rewrite /triggerUB SBRed.unwrapU.
-      ired; rewrite !bind_trigger. gstep. econs. i. ss.
-  }
-  {
-    rewrite! SBRed.yield. rewrite! bind_trigger.
-    gstep. econs. i. r. gbase. eauto.
-  }
-  {
-    rewrite! SBRed.gettid. rewrite! bind_trigger.
-    gstep. econs. i. r. gbase. eauto.
-  }
-  destruct s; [destruct p|].
-  {
-    rewrite! SBRed.put. des_ifs.
-    + rewrite SBRed.put. des_ifs.
-      * rewrite! bind_trigger. gstep. econs. i. r. gbase. eauto.
-      * exfalso. eapply existsb_exists in Heq. des. eapply SCP in Heq.
-        assert (XEQ:=existsb_exists).
-        hdes. rewrite XEQ1 in Heq0; ss; eauto.
-    + rewrite /triggerUB SBRed.unwrapU.
-      ired; rewrite !bind_trigger. gstep. econs. i. ss.
-  }
-  {
-    rewrite! SBRed.get. des_ifs.
-    + rewrite! SBRed.get. des_ifs.
-      * rewrite! bind_trigger. gstep. econs. i. r. gbase. eauto.
-      * exfalso. eapply existsb_exists in Heq. des. eapply SCP in Heq.
-        assert (XEQ:=existsb_exists).
-        hdes. rewrite XEQ1 in Heq0; ss; eauto.
-    + rewrite /triggerUB SBRed.unwrapU.
-      ired; rewrite !bind_trigger. gstep. econs. i. ss.
-  }
-  {
-    destruct c.
-    - rewrite! SBRed.choose. rewrite! bind_trigger.
-      gstep. econs. i. r. gbase. eauto.
-    - rewrite !SBRed.take !bind_trigger.
-      destruct (excluded_middle_informative _) eqn: E; s.
-      + rewrite orb_true_r SBRed.take E orb_true_r.
-        gstep. r; s. econs. i. ired. gbase. eauto.
-      + destruct img0; s.
-        * rewrite SBRed.take. destruct img1; s.
-          { gstep. r; s. econs. i. ired. gbase. et. }
-          { exploit IMPL; et; i. inv x0. }
-        * rewrite SBRed.vis_take. des_ifs.
-          { gstep. r; s. econs. ss. }
-          { gstep. r; s. econs. ss. }
-    - rewrite! SBRed.io. rewrite! bind_trigger.
-      gstep. econs. i. r. gbase. eauto.
-  }
-Qed.
-
-Lemma inv_sandbox_tau `{Σ: GRA} {X} img msk sc (itr : itree crisE X)
-    (SB : SB.sandbox img msk sc (tau;; itr) = tau;; itr) :
-  SB.sandbox img msk sc itr = itr.
-Proof.
-  rewrite SBRed.tau in SB. inv SB.
-  rewrite sandbox_well_scoped; ss.
-0Qed.
-
-Lemma inv_sandbox_core `{Σ: GRA} {X Y} x img msk sc (ktr : X -> itree crisE Y) (e: coreE X)
-    (SB : SB.sandbox img msk sc (trigger e >>= ktr) = trigger e >>= ktr) :
-  SB.sandbox img msk sc (ktr x) = ktr x.
-Proof.
-  destruct e.
-  - rewrite SBRed.bind SBRed.choose in SB.
-    rewrite! bind_trigger in SB. inv SB.
-    eapply inj_pair2, equal_f in H0. eauto.
-  - rewrite SBRed.bind SBRed.take in SB. des_ifs.
-    + rewrite! bind_trigger in SB. inv SB.
-      eapply inj_pair2, equal_f in H0. eauto.
-    + bsimpl. des; subst; ss.
-      rewrite !bind_trigger bind_vis in SB. depdes SB.
-      exfalso. destruct (excluded_middle_informative _); ss.
-  - rewrite SBRed.bind SBRed.io in SB.
-    rewrite! bind_trigger in SB. inv SB.
-    eapply inj_pair2, equal_f in H0. eauto.
-Qed.
-
-
-Lemma inv_sandbox_spawn `{Σ: GRA} {Y} x img msk sc (ktr : _ -> itree crisE Y) f a
-    (SB : SB.sandbox img msk sc (trigger (Spawn f a) >>= ktr) = trigger (Spawn f a) >>= ktr) :
-  SB.sandbox img msk sc (ktr x) = ktr x.
-Proof.
-  rewrite SBRed.bind SBRed.spawn in SB.
-  des_ifs; rewrite! bind_trigger in SB; depdes SB.
-  - eapply equal_f in x. eauto.
-  - rewrite bind_bind bind_vis in x. depdes x.
-Qed.
-
-Lemma inv_sandbox_gettid `{Σ : GRA} {Y} x img msk sc (ktr : _ -> itree crisE Y)
-    (SB : SB.sandbox img msk sc (trigger GetTid >>= ktr) = trigger GetTid >>= ktr) :
-  SB.sandbox img msk sc (ktr x) = ktr x.
-Proof.
-  rewrite SBRed.bind SBRed.gettid in SB.
-  des_ifs; rewrite! bind_trigger in SB; depdes SB.
-  - eapply equal_f in x. eauto.
-Qed.
-
-Lemma inv_sandbox_pg `{Σ: GRA} {X Y} x img msk sc (ktr : X -> itree crisE Y) (pg : pgE X)
-    (SB : SB.sandbox img msk sc (trigger pg >>= ktr) = trigger pg >>= ktr) :
-  SB.sandbox img msk sc (ktr x) = ktr x.
-Proof.
-  destruct pg.
-  { rewrite SBRed.bind SBRed.put in SB.
-    des_ifs; rewrite! bind_trigger in SB; depdes SB.
-    - eapply equal_f in x. eauto.
-    - rewrite bind_bind bind_vis in x. depdes x.
-  }
-  { rewrite SBRed.bind SBRed.get in SB.
-    des_ifs; rewrite! bind_trigger in SB; depdes SB.
-    - eapply equal_f in x. eauto.
-    - rewrite bind_bind bind_vis in x. depdes x.
-  }
-Qed.
-
-Lemma inv_sandbox_ag `{Σ: GRA} {X R} x img msk sc (ktr : X -> itree crisE R) (e: agE X)
-    (SB : SB.sandbox img msk sc (trigger e >>= ktr) = trigger e >>= ktr) :
-  SB.sandbox img msk sc (ktr x) = ktr x.
-Proof.
-  destruct e.
-  - rewrite SBRed.bind SBRed.Assume in SB. des_ifs.
-    + rewrite! bind_trigger in SB. inv SB.
-      eapply inj_pair2, equal_f in H0. eauto.
-    + rewrite !bind_trigger bind_vis in SB. depdes SB.
-  - rewrite SBRed.bind SBRed.AssumeRes in SB.
-    rewrite! bind_trigger in SB. inv SB.
-    eapply inj_pair2, equal_f in H0. eauto.
-  - rewrite SBRed.bind SBRed.Guarantee in SB.
-    rewrite! bind_trigger in SB. inv SB.
-    eapply inj_pair2, equal_f in H0. eauto.
-Qed.
-
-Lemma alist_upd_not_exists k v st scopes
-    (NOTEXT : existsb (String.eqb k.1) scopes = false)
-    (INSCP : incl (state_scopes st) scopes) :
-  alist_upd k v st = st.
-Proof.
-  eapply alist_upd_not_in.
-  ii. eapply in_map with (f:=fst) in H.
-  rewrite List.map_map in H. eapply INSCP in H.
-  assert (∃x, In x scopes /\ String.eqb k.1 x = true).
-  { exists k.1. esplits; [eauto|]. eapply String.eqb_refl. }
-  eapply existsb_exists in H0. clarify.
-Qed.
-
-Lemma alist_find_existsb st scopes k v
-    (INSCP : incl (state_scopes st) scopes)
-    (FIND : alist_find k st = Some v) :
-  existsb (String.eqb k.1) scopes = true.
-Proof.
-  eapply existsb_exists.
-  eapply alist_find_fst_some, in_map in FIND.
-  rewrite List.map_map in FIND.
-  exists k.1. esplits; eauto. eapply String.eqb_refl.
-Qed.
-
-Lemma alist_find_not_exists st scopes k
-    (INSCP : incl (state_scopes st) scopes)
-    (NOTEXT : existsb (String.eqb k.1) scopes = false) :
-  alist_find k st = None.
-Proof.
-  eapply alist_find_fst_notin.
-  ii. eapply in_map with (f:=fst) in H.
-  rewrite List.map_map in H. eapply INSCP in H.
-  assert (∃x, In x scopes /\ String.eqb k.1 x = true).
-  { exists k.1. esplits; [eauto|]. eapply String.eqb_refl. }
-  eapply existsb_exists in H0. clarify.
-Qed.
-
-Lemma alist_find_exists_l st ctx scopeS scopeC (k : key)
-    (DISJ : List.NoDup (scopeS ++ scopeC))
-    (INS : incl (state_scopes st) scopeS)
-    (INC : incl (state_scopes ctx) scopeC)
-    (EXT : existsb (String.eqb k.1) scopeS = true) :
-  alist_find k (st ++ ctx) = alist_find k st.
-Proof.
-  rewrite alist_find_app_o. des_ifs.
-  eapply alist_find_fst_notin. ii.
-  eapply existsb_exists in EXT. des.
-  eapply NoDup_app_disjoint; eauto.
-  eapply INC. unfold state_scopes. rewrite -List.map_map.
-  eapply in_map with (f:=fst) in H.
-  eapply String.eqb_eq in EXT0. subst. eauto.
-Qed.
-
-Lemma wf_eq_solve `{Σ: GRA} (a b : Σ) : ✓ a -> a = b -> ✓ b.
-Proof. i. rewrite <- H0. eauto. Qed.
-
-Lemma wf_inv_l `{Σ: GRA} ms0 ms1
-    (WF : Mod.wf (Mod.add ms0 ms1)) :
-  Mod.wf ms0.
-Proof.
-  inv WF; ss. rewrite map_app in wf_fns.
-  econs; eauto using nodup_app_l.
-Qed.
 
 Ltac mstep := guclo msimC_spec; econs; econs; eauto; econs; eauto.
 
-Lemma msim_ctx
-    `{Σ: GRA} contextual fnsems_src fnsems_tgt (fl_src fl_tgt fl_ctx: alist (option string) _)
-    Ist (img : bool) (msk : _ -> bool) scp scpC RR
-    (FLS : fl_src = (List.map (map_snd SB.sandbox_body) fnsems_src))
-    (FLT : fl_tgt = (List.map (map_snd SB.sandbox_body) fnsems_tgt))
-    (WS : ∀ fn img0 msk0 scp0 bd0 (IN : alist_find (Some fn) fnsems_src = Some (img0,msk0,scp0,bd0)), (img0 → img) ∧ (∀ fn, msk0 fn → msk fn) ∧ incl scp0 scp)
-    (WT : ∀ fn img0 msk0 scp0 bd0 (IN : alist_find (Some fn) fnsems_tgt = Some (img0,msk0,scp0,bd0)), (img0 → img) ∧ (∀ fn, msk0 fn → msk fn) ∧ incl scp0 scp)
-    (DISJ : List.NoDup (scp ++ scpC))
-
-    ps pt st_src st_tgt st_ctx itr_src itr_tgt fmr
-    (SCPT : incl (state_scopes st_tgt) scp)
-    (SCPS : incl (state_scopes st_src) scp)
-    (SCPC : incl (state_scopes st_ctx) scpC)
-    (ITRT : SB.sandbox img msk scp itr_tgt = itr_tgt)
-    (ITRS : SB.sandbox img msk scp itr_src = itr_src)
-    (SIM : msim open fl_src fl_tgt Ist (ist_with_eq RR) ps pt
-             (st_src, itr_src) (st_tgt, itr_tgt) fmr)
-  :
-  @msim _ contextual (fl_src ++ fl_ctx) (fl_tgt ++ fl_ctx)
-    (IstProd (IstSB scp Ist) (IstSB scpC IstEq)) Any.t Any.t
-    (ist_with_eq (IstProd (IstSB scp RR) (IstSB scpC IstEq))) ps pt
-    (st_src ++ st_ctx, itr_src) (st_tgt ++ st_ctx, itr_tgt) fmr.
-  Proof.
-    guardH FLS. guardH FLT. hdes.
-    move WS0 at top. move WS2 at top. move WS3 at top.
-    move WT0 at top. move WT2 at top. move WT3 at top.
-    ginit. s. revert_until DISJ. gcofix CIH. i.
-    remember (st_src, itr_src). remember (st_tgt, itr_tgt).
-    move SIM before CIH. revert_until SIM. punfold SIM.
-    pattern ps, pt, p, p0, fmr.
-    eapply _msim_tarski, SIM; i. clear SIM fmr. rename fmr0 into fmr.
-    guclo msim_wfC_spec. econs. i.
-    guclo msim_nodupC_spec. econs. i.
-    exploit IN; i; des; eauto.
-    { rewrite map_app in NODFS. eapply NoDup_app_remove_r. eauto. }
-    { rewrite map_app in NODFT. eapply NoDup_app_remove_r. eauto. }
-    { subst. rewrite map_app in NODS. eapply NoDup_app_remove_r. eauto. }
-    { subst. rewrite map_app in NODT. eapply NoDup_app_remove_r. eauto. }
-    clear IN. destruct x0; i; des; inv Heqp; try inv Heqp0.
-    - mstep. iIntros "H". rewrite RET. iMod "H" as "[% H]". subst.
-      iModIntro. iSplit; eauto. iExists st_src, st_tgt, st_ctx, st_ctx.
-      repeat (iSplit; et).
-    - mstep.
-      { instantiate (1:= FR). iIntros "H". iPoseProof (INV with "H") as ">[H FR]".
-        iModIntro. iFrame. iExists st_ctx, st_ctx.
-        iSplit; eauto.
-      }
-      i. guclo msim_wfC_spec. econs. i.
-      eapply Own_bupd_split in INV0; eauto. des.
-      eapply Own_general_soundness in INV1; eauto; cycle 1.
-      { by eapply Own_wand_valid; first by iIntros "F"; iMod (INV0 with "F") as "[? _]"; iFrame. }
-      rewrite /IstProd in INV1. uPred.unseal_in INV1; destruct INV1 as [st_srcL [st_tgtL [st_srcR [st_tgtR INV1]]]].
-      destruct INV1 as [a1' [a1'' [INV1 [INV1' INV1'']]]]; inv INV1'.
-      rewrite /IstSB in INV1''; rr in INV1''; uPred.unseal_in INV1''; des.
-      destruct INV1''0 as [x0' [x0'' [? [INV1''0 ?]]]]; inv INV1''0.
-      destruct INV1''1 as [x1' [x1'' [? [INV1''1 ?]]]]; inv INV1''1.
-      rewrite /IstEq in H7; uPred.unseal_in H7; inv H7.
-      (*
-        new states after call should maintain the scope of previous states.
-        ctx state should maintain its own scope.
-      *)
-      eapply K; try refl; eauto using inv_sandbox_event; try nia; cycle 3.
-      { eapply nodup_app_l. rewrite <- map_app. eauto. }
-      { eapply nodup_app_l. rewrite <- map_app. eauto. }
-      iIntros "H". iPoseProof (INV0 with "H") as ">H".
-      iDestruct "H" as "[H1 H2]"; iModIntro; iSplitL "H1".
-      { rewrite INV1 INV1'' H2; iDestruct "H1" as "[_ [[_ H] _]]";
-          iPoseProof (Own_general_completeness with "H") as "H"; eauto. }
-      { iApply INV2; done. }
-    - mstep. i. eapply K; try refl; eauto using inv_sandbox_core.
-    - mstep. { rewrite alist_find_app_o. rewrite FUN. eauto. }
-      eapply K; try refl; eauto. grind.
-      rewrite! SBRed.bind.
-      move FLS at bottom. move FUN at bottom.
-      rewrite FLS in FUN.
-      rewrite alist_find_map_snd in FUN.
-      unfold o_map in FUN. des_ifs. unfold SB.sandbox_body.
-      destruct f0 as [[[img0 msk0] scp0] bd0]. s.
-      rewrite sandbox_well_scoped; eauto; cycle 1.
-      f_equal. extensionalities.
-      rewrite ?SBRed.bind !SBRed.tau SBRed.ret.
-      do 4 f_equal. extensionalities. eapply inv_sandbox_event; eauto.
-    - mstep. { rewrite alist_find_app_o. rewrite FUN. eauto. }
-      eapply K; try refl; eauto. grind.
-      rewrite! SBRed.bind.
-      move FLT at bottom. move FUN at bottom.
-      rewrite FLT in FUN.
-      rewrite alist_find_map_snd in FUN.
-      unfold o_map in FUN. des_ifs. unfold SB.sandbox_body.
-      destruct f0 as [[[img0 msk0] scp0] bd0]. s.
-      rewrite sandbox_well_scoped; eauto.
-      f_equal. extensionalities.
-      rewrite ?SBRed.bind !SBRed.tau SBRed.ret.
-      do 4 f_equal. extensionalities. eapply inv_sandbox_event; eauto.
-    - mstep. eapply K; try refl; eauto using inv_sandbox_tau.
-    - mstep. eapply K; try refl; eauto using inv_sandbox_tau.
-    - mstep. i. eapply K; try refl; eauto using inv_sandbox_core.
-    - mstep. i. eapply K; try refl; eauto using inv_sandbox_core.
-    - mstep. eapply K; try refl; eauto using inv_sandbox_core.
-    - mstep. eapply K; try refl; eauto using inv_sandbox_core.
-
-    - assert (H1:= ITRS).
-      rewrite  -ITRS SBRed.bind SBRed.put. des_ifs.
-      + mstep.
-        assert (UPD : alist_upd k v (st_src ++ st_ctx) = alist_upd k v st_src ++ st_ctx).
-        {
-          move SCPS at bottom. move SCPC at bottom.
-          eapply existsb_exists in Heq. des. eapply String.eqb_eq in Heq0.
-          rewrite alist_upd_not_tail; eauto.
-          ii. eapply NoDup_app_disjoint; eauto.
-          eapply in_map with (f:=fst) in H2.
-          rewrite List.map_map in H2. eapply SCPC in H2.
-          rewrite <- Heq0. eauto.
-        }
-        rewrite UPD. eapply K; try refl; eauto.
-        { rewrite state_scopes_update. eauto. }
-        { eapply sandbox_well_scoped; et; refl. }
-        { f_equal. symmetry. eapply inv_sandbox_pg. eauto. }
-      + unfold triggerUB. ired. mstep. ss.
-
-  - assert (H1:=ITRT).
-    rewrite -ITRT SBRed.bind SBRed.put. des_ifs.
-    + mstep.
-      assert (UPD : alist_upd k v (st_tgt ++ st_ctx) = alist_upd k v st_tgt ++ st_ctx).
-      {
-        move SCPS at bottom. move SCPC at bottom.
-        eapply existsb_exists in Heq. des. eapply String.eqb_eq in Heq0.
-        eapply alist_upd_not_tail. eauto.
-        ii. eapply NoDup_app_disjoint; eauto.
-        eapply in_map with (f:=fst) in H2.
-        rewrite List.map_map in H2. eapply SCPC in H2.
-        rewrite <- Heq0. eauto.
-      }
-      rewrite UPD. eapply K; try refl; eauto.
-      { rewrite state_scopes_update. eauto. }
-      { eapply sandbox_well_scoped; et. refl. }
-      { f_equal. symmetry. eapply inv_sandbox_pg. eauto. }
-    + rewrite SBRed.bind SBRed.put Heq !bind_trigger in H1.
-      exfalso. unfold triggerUB in H1. rewrite bind_bind bind_vis in H1. ss.
-
-  - assert (H1:=ITRS).
-    rewrite  -ITRS SBRed.bind SBRed.get. des_ifs.
-    + mstep. eapply K; try refl; eauto.
-      { eapply sandbox_well_scoped; et. refl. }
-      erewrite alist_find_exists_l; eauto.
-      repeat f_equal. symmetry. eapply inv_sandbox_pg; eauto.
-    + unfold triggerUB. ired. mstep. ss.
-
-  - assert (H1:=ITRT).
-    rewrite  -ITRT SBRed.bind SBRed.get. des_ifs.
-    + mstep. eapply K; try refl; eauto.
-      { eapply sandbox_well_scoped; et. refl. }
-      erewrite alist_find_exists_l; eauto.
-      repeat f_equal. symmetry. eapply inv_sandbox_pg; eauto.
-    + rewrite SBRed.bind SBRed.get Heq !bind_trigger in H1.
-      exfalso. unfold triggerUB in H1. rewrite bind_bind bind_vis in H1. ss.
-
-  - mstep. i. eapply K; try refl; eauto using inv_sandbox_ag.
-  - mstep. i. eapply K; try refl; eauto using inv_sandbox_ag.
-  - mstep. i. eapply K; try refl; eauto using inv_sandbox_ag.
-  - mstep. i. eapply K; try refl; eauto using inv_sandbox_ag.
-  - mstep. i. eapply K; try refl; eauto using inv_sandbox_ag.
-  - mstep. i. eapply (K fmr1); et; i; des.
-    try refl; eauto using inv_sandbox_ag.
-  (* - guclo @msimC_spec. econs; esplits; et.
-    eapply msim_assume_res_both; et.
-    i. eapply K; try refl; eauto using inv_sandbox_ag. *)
-  - mstep. intros tid; eapply (K tid); try refl; eauto.
-    + eapply inv_sandbox_spawn in ITRT. eauto.
-    + eapply inv_sandbox_spawn in ITRS. eauto.
-  - mstep.
-    { instantiate (1:= FR). iIntros "H". iPoseProof (INV with "H") as ">[H FR]".
-      iModIntro. iFrame. iExists st_ctx, st_ctx.
-      iSplit; eauto.
-    }
-    i. guclo msim_wfC_spec. econs. i.
-    eapply Own_bupd_split in INV0; eauto. des.
-    eapply Own_general_soundness in INV1; eauto; cycle 1.
-    { by eapply Own_wand_valid; first by iIntros "F"; iMod (INV0 with "F") as "[? _]"; iFrame. }
-    rewrite /IstProd in INV1. uPred.unseal_in INV1; destruct INV1 as [st_srcL [st_tgtL [st_srcR [st_tgtR INV1]]]].
-    destruct INV1 as [a1' [a1'' [INV1 [INV1' INV1'']]]]; inv INV1'.
-    rewrite /IstSB in INV1''; rr in INV1''; uPred.unseal_in INV1''; des.
-    destruct INV1''0 as [x0' [x0'' [? [INV1''0 ?]]]]; inv INV1''0.
-    destruct INV1''1 as [x1' [x1'' [? [INV1''1 ?]]]]; inv INV1''1.
-    rewrite /IstEq in H7; uPred.unseal_in H7; inv H7.
-    (*
-      new states after call should maintain the scope of previous states.
-      ctx state should maintain its own scope.
-    *)
-    eapply K; try refl; eauto; try nia; cycle 3.
-    { rewrite SBRed.bind SBRed.yield !bind_trigger in ITRT.
-      depdes ITRT. eapply equal_f in x. eauto. }
-    { rewrite SBRed.bind SBRed.yield !bind_trigger in ITRS.
-      depdes ITRS. eapply equal_f in x. eauto. }
-    { eapply nodup_app_l. rewrite <- map_app. eauto. }
-    { eapply nodup_app_l. rewrite <- map_app. eauto. }
-    iIntros "H". iPoseProof (INV0 with "H") as ">H".
-    iDestruct "H" as "[H1 H2]"; iModIntro; iSplitL "H1".
-    { rewrite INV1 INV1'' H2; iDestruct "H1" as "[_ [[_ H] _]]";
-        iPoseProof (Own_general_completeness with "H") as "H"; eauto. }
-    { iApply INV2; done. }
-
-  - mstep. intros tid; eapply (K tid); try refl; eauto.
-    + eapply inv_sandbox_gettid in ITRT. eauto.
-    + eapply inv_sandbox_gettid in ITRS. eauto.
-
-  - gstep. econs. econs. econs; eauto. econs; eauto.
-    gbase. pclearbot. eapply CIH; try refl; eauto.
-Qed.
-
- *)
-Ltac mstep := guclo msimC_spec; econs; econs; eauto; econs; eauto.
-
-Local Lemma Own_Ist `{Σ : GRA} FR fmr scp Ist st_src st_tgt :
+Local Lemma Own_Ist `{Σ : GRA} FR fmr scp scp_ctx Ist st_src st_tgt :
   ✓ fmr →
-  (Own fmr ⊢ |==> IstProd (IstSB scp Ist) IstEq st_src st_tgt ∗ FR) →
+  (Own fmr ⊢ |==> IstProd (IstSB scp Ist) (IstSB scp_ctx IstEq) st_src st_tgt ∗ FR) →
   ∃ st_srcL st_tgtL st_ctx,
     st_src = union_with (const (const (Some None))) st_srcL st_ctx ∧
     st_tgt = union_with (const (const (Some None))) st_tgtL st_ctx ∧
     (elements (dom st_srcL)).*1 ⊆ scp ∧
     (elements (dom st_tgtL)).*1 ⊆ scp ∧
+    (elements (dom st_ctx)).*1 ⊆ scp_ctx ∧
     (Own fmr ⊢ |==> Ist st_srcL st_tgtL ∗ FR).
 Proof.
   intros Hfmr2val Hfmr2.
@@ -527,35 +75,35 @@ Proof.
   rewrite /IstProd /IstSB /IstEq in Hfmr21; uPred.unseal_in Hfmr21.
   destruct Hfmr21 as [st_srcL [st_tgtL [st_srcR [st_tgtR Hfmr21]]]].    
   destruct Hfmr21 as [? [fmr212 [Hfmr21 [[-> ->] Hfmr212]]]].
-  destruct Hfmr212 as [fmr2121 [? [Hfmr212 [[? [? [Hfmr2121 [[? ?] Hfmr21211]]]] ->]]]].
-  eapply Own_general_completeness in Hfmr21211.
+  destruct Hfmr212 as [fmr2121 [fmr2122 [Hfmr212 [Hfmr2121 Hfmr2122]]]].
+  destruct Hfmr2121 as [? [fmr21212 [Hfmr2121 [[?] Hfmr21212]]]].
+  destruct Hfmr2122 as [? [? [Hfmr2122 [[?] []]]]].
+  eapply Own_general_completeness in Hfmr21212.
   esplits; eauto.
-  rewrite Hfmr2 Hfmr21 Hfmr212 Hfmr2121 ?Own_op Hfmr21211 Hfmr22.
+  rewrite Hfmr2 Hfmr21 Hfmr212 Hfmr2121 ?Own_op Hfmr21212 Hfmr22.
   iIntros "> [[? [[? ?] ?]] ?]"; by iFrame.
 Qed.
 
+Definition msk_scp `{Σ : GRA} (scp : list string) : emask :=
+  λ X e,
+    match e with
+    | inl1 _ => true
+    | inr1 (inl1 _) => true
+    | inr1 (inr1 (inl1 (SPut k v))) => decide (k.1 ∈ scp)
+    | inr1 (inr1 (inl1 (SGet k))) => decide (k.1 ∈ scp)
+    | inr1 (inr1 (inr1 _)) => true
+    end.
+
 Lemma msim_ctx
     `{Σ : GRA} contextual ms mt ctx
-    Ist RR scp msk
-    (* (img : bool) (msk : _ -> bool) scp scpC  *)
-    ps pt st_src st_tgt st_ctx itr_src itr_tgt fmr
-    (* (WS : ∀ fn img0 msk0 scp0 bd0 (IN : alist_find (Some fn) fnsems_src = Some (img0,msk0,scp0,bd0)),
-      (img0 → img) ∧ (∀ fn, msk0 fn → msk fn) ∧ incl scp0 scp)
-    (WT : ∀ fn img0 msk0 scp0 bd0 (IN : alist_find (Some fn) fnsems_tgt = Some (img0,msk0,scp0,bd0)),
-      (img0 → img) ∧ (∀ fn, msk0 fn → msk fn) ∧ incl scp0 scp)
-    (DISJ : List.NoDup (scp ++ scpC)) *)
-
-    
-    (* (SCPT : incl (state_scopes st_tgt) scp)
-    (SCPS : incl (state_scopes st_src) scp)
-    (SCPC : incl (state_scopes st_ctx) scpC)
-    (ITRT : SB.sandbox img msk scp itr_tgt = itr_tgt)
-    (ITRS : SB.sandbox img msk scp itr_src = itr_src) *)
-  :
-  (elements (dom st_src)).*1 ⊆ scp →
-  (elements (dom st_tgt)).*1 ⊆ scp →
-  SB.sandbox msk itr_src = itr_src →
-  SB.sandbox msk itr_tgt = itr_tgt →
+    Ist RR
+    ps pt st_src st_tgt st_ctx itr_src itr_tgt fmr :
+  Mod.scopes ms ⊆+ Mod.scopes mt →
+  (elements (dom st_src)).*1 ⊆ (Mod.scopes mt) →
+  (elements (dom st_tgt)).*1 ⊆ (Mod.scopes mt) →
+  (elements (dom st_ctx)).*1 ⊆ (Mod.scopes ctx) →
+  SB.sandbox (msk_scp (Mod.scopes mt)) itr_src = itr_src →
+  SB.sandbox (msk_scp (Mod.scopes mt)) itr_tgt = itr_tgt →
   Mod.wf (ms ★ ctx) →
   Mod.wf (mt ★ ctx) →
   msim open
@@ -565,21 +113,20 @@ Lemma msim_ctx
   @msim _ contextual
     ((λ v : option _, SB.sandbox_body <$> v) <$> (Mod.fnsems (ms ★ ctx)))
     ((λ v : option _, SB.sandbox_body <$> v) <$> (Mod.fnsems (mt ★ ctx)))
-    (IstProd (IstSB scp Ist) IstEq) Any.t Any.t
-    (ist_with_eq (IstProd (IstSB scp RR) IstEq)) ps pt
+    (IstProd (IstSB (Mod.scopes mt) Ist) (IstSB (Mod.scopes ctx) IstEq)) Any.t Any.t
+    (ist_with_eq (IstProd (IstSB (Mod.scopes mt) RR) (IstSB (Mod.scopes ctx) IstEq))) ps pt
     (union_with (const (const (Some None))) st_src st_ctx, itr_src) 
     (union_with (const (const (Some None))) st_tgt st_ctx, itr_tgt) fmr.
 Proof.
-  (* guardH FLS. guardH FLT. hdes. *)
-  (* move WS0 at top. move WS2 at top. move WS3 at top. *)
-  (* move WT0 at top. move WT2 at top. move WT3 at top. *)
-  ginit. intros ???? Hwfs Hwft; move Hwfs at top; move Hwft at top.
-  revert_until msk. gcofix CIH.
-  intros ps pt st_src st_tgt st_ctx itr_src itr_tgt fmr ? ? Hsbs Hsbt Hsim.
+  ginit.
+  intros ?????? Hwfs Hwft.
+  move Hwfs at top. move Hwft at top.
+  revert_until RR. gcofix CIH.
+  intros ps pt st_src st_tgt st_ctx itr_src itr_tgt fmr Hscopest ? ? ? Hsbs Hsbt Hsim.
   remember (st_src, itr_src) as ss. remember (st_tgt, itr_tgt) as st.
   move Hsim before CIH. revert_until Hsim. punfold Hsim.
   pattern ps, pt, ss, st, fmr.
-  eapply _msim_tarski, Hsim; clear Hsim fmr; intros ???? fmr Hin ????? ???? -> ->.
+  eapply _msim_tarski, Hsim; clear Hsim fmr; intros ???? fmr Hin ????? ?????? -> ->.
   guclo msim_wfC_spec. econs. intros Hval.
   guclo msim_nodupC_spec; econs; intros Hfs Hft Hss Hst; hexploit Hin; ss.
   { move: Hfs; rewrite ?map_Forall_lookup => Hfs i x; move: Hfs => /(_ i x) /=.
@@ -601,248 +148,118 @@ Proof.
 
   clear Hin; intros Hin.
   destruct Hin as [fmr1 [Hin Hfmr]]; eauto.
-  inv Hin; try by (mstep; eauto using inv_sandbox_event, inv_sandbox_tau).
+  inv Hin; try by (mstep; eauto using inv_sandbox_ktr, inv_sandbox_tau).
   { mstep; rewrite RET; iIntros "> [-> $] !>"; iSplit; [done|iExists _, _; iSplit; eauto]. }
   { mstep.
     { instantiate (1:=FR). rewrite INV; iIntros "> [$ $] !>"; iExists _, _; iSplit; eauto. }
     intros ? st_src2 st_tgt2 fmr2 Hfmr2.
     guclo msim_wfC_spec; econs; intros Hfmr2val.
-    hexploit Own_Ist; eauto; intros [? [? [? [-> [-> [? [? Hfmr22]]]]]]].
-    eapply K; eauto using inv_sandbox_event.
+    hexploit Own_Ist; eauto; intros [? [? [? [-> [-> [? [? [? ?]]]]]]]].
+    eapply K; eauto using inv_sandbox_ktr.
   }
   { mstep; cycle 1.
-    { eapply K; eauto using inv_sandbox_event.
+    { eapply K; eauto using inv_sandbox_ktr.
       ired. rewrite SBRed.bind; ired.
-      assert (SB.sandbox msk (f varg) = f varg).
-      { admit. }
-      rewrite H2; grind.
-      rewrite SBRed.tau; ired; grind; eauto using inv_sandbox_event.
+      assert (Hf : SB.sandbox (msk_scp (Mod.scopes mt)) (f varg) = f varg).
+      { move: FUN; rewrite lookup_fmap; destruct (_ ms !! _) as [[[fnmsk ?]|]|] eqn : Hfn; ss.
+        i; clarify; eapply sandbox_well_scoped; eauto.
+        intros ? e; depdes e; ss. depdes s; ss. depdes s; ss.
+        depdes p; ss; hexploit (Mod.well_scoped_fns ms); rewrite map_Forall_lookup =>
+          /(_ (Some fn) (fnmsk, f0)); rewrite lookup_omap Hfn => /(_ eq_refl);
+          [intros [Hkey ?]|intros [? Hkey]] => /Hkey; case_decide; ss;
+          intros Hin; eapply elem_of_submseteq in Hin; eauto.
+      }
+      rewrite Hf; grind.
+      rewrite SBRed.tau; ired; grind; eauto using inv_sandbox_ktr.
     }
-    admit.
+    revert FUN; intros [[f2|] [? FUN]]%lookup_fmap_Some; ss; clarify.
+    move : FUN => /(Mod.lookup_add_l); move /(_ ctx Hwfs) => /=; rewrite lookup_fmap => -> //=.
   }
-  { admit. }
-  { admit. }
-  { admit. }
-  { admit. }
-  { admit. }
+  { mstep; cycle 1.
+    { eapply K; eauto using inv_sandbox_ktr.
+      ired. rewrite SBRed.bind; ired.
+      assert (Hf : SB.sandbox (msk_scp (Mod.scopes mt)) (f varg) = f varg).
+      { move: FUN; rewrite lookup_fmap; destruct (_ mt !! _) as [[[fnmsk ?]|]|] eqn : Hfn; ss.
+        i; clarify; eapply sandbox_well_scoped; eauto.
+        intros ? e; depdes e; ss. depdes s; ss. depdes s; ss.
+        depdes p; ss; hexploit (Mod.well_scoped_fns mt); rewrite map_Forall_lookup =>
+          /(_ (Some fn) (fnmsk, f0)); rewrite lookup_omap Hfn => /(_ eq_refl);
+          [intros [Hkey ?]|intros [? Hkey]] => /Hkey; case_decide; ss;
+          intros Hin; eapply elem_of_submseteq in Hin; eauto.
+      }
+      rewrite Hf; grind.
+      rewrite SBRed.tau; ired; grind; eauto using inv_sandbox_ktr.
+    }
+    revert FUN; intros [[f2|] [? FUN]]%lookup_fmap_Some; ss; clarify.
+    move : FUN => /(Mod.lookup_add_l); move /(_ ctx Hwft) => /=; rewrite lookup_fmap => -> //=.
+  }
+  { mstep.
+    eapply inv_sandbox_event in Hsbs as [Hktr Hmsk]; ss; case_decide; ss.
+    rewrite insert_union_with_l.
+    { eapply K; eauto. rewrite dom_insert_L; set_solver. }
+    rewrite not_elem_of_dom_1 //.
+    assert (Mod.scopes ctx ## Mod.scopes mt); [|set_solver].
+    hexploit (Mod.wf_scopes _ Hwft); eauto => /NoDup_app; i; des; set_solver.
+  }
+  { mstep.
+    eapply inv_sandbox_event in Hsbt as [Hktr Hmsk]; ss; case_decide; ss.
+    rewrite insert_union_with_l.
+    { eapply K; eauto. rewrite dom_insert_L; set_solver. }
+    rewrite not_elem_of_dom_1 //.
+    assert (Mod.scopes ctx ## Mod.scopes mt); [|set_solver].
+    hexploit (Mod.wf_scopes _ Hwft); eauto => /NoDup_app; i; des; set_solver.
+  }
+  { mstep. eapply K; eauto using inv_sandbox_ktr.
+    eapply inv_sandbox_event in Hsbs as [Hktr Hmsk]; ss; case_decide; ss.
+    rewrite lookup_union_with (not_elem_of_dom_1 st_ctx); [destruct (_ !! _); ss|].
+    assert (Mod.scopes ctx ## Mod.scopes mt); [|set_solver].
+    hexploit (Mod.wf_scopes _ Hwft); eauto => /NoDup_app; i; des; set_solver.
+  }
+  { mstep. eapply K; eauto using inv_sandbox_ktr.
+    eapply inv_sandbox_event in Hsbt as [Hktr Hmsk]; ss; case_decide; ss.
+    rewrite lookup_union_with (not_elem_of_dom_1 st_ctx); [destruct (_ !! _); ss|].
+    assert (Mod.scopes ctx ## Mod.scopes mt); [|set_solver].
+    hexploit (Mod.wf_scopes _ Hwft); eauto => /NoDup_app; i; des; set_solver.
+  }
   { mstep.
     { instantiate (1:=FR). rewrite INV; iIntros "> [$ $] !>"; iExists _, _; iSplit; eauto. }
     intros st_src2 st_tgt2 fmr2 Hfmr2.
     guclo msim_wfC_spec; econs; intros Hfmr2val.
-    hexploit Own_Ist; eauto; intros [? [? [? [-> [-> [? [? Hfmr22]]]]]]].
-    eapply K; eauto using inv_sandbox_event.
+    hexploit Own_Ist; eauto; intros [? [? [? [-> [-> [? [? [? ?]]]]]]]].
+    eapply K; eauto using inv_sandbox_ktr.
   }
   { gstep. econs. econs. econs; eauto. econs; eauto.
     gbase. pclearbot. eapply CIH; try refl; eauto.
   }
+  Unshelve. all: try exact (()↑).
+Qed.
 
-    (* destruct x0; i; des; inv Heqp; try inv Heqp0.
-    - mstep. iIntros "H". rewrite RET. iMod "H" as "[% H]". subst.
-      iModIntro. iSplit; eauto. iExists st_src, st_tgt, st_ctx, st_ctx.
-      repeat (iSplit; et).
-    - mstep.
-      { instantiate (1:= FR). iIntros "H". iPoseProof (INV with "H") as ">[H FR]".
-        iModIntro. iFrame. iExists st_ctx, st_ctx.
-        iSplit; eauto.
-      }
-      i. guclo msim_wfC_spec. econs. i.
-      eapply Own_bupd_split in INV0; eauto. des.
-      eapply Own_general_soundness in INV1; eauto; cycle 1.
-      { by eapply Own_wand_valid; first by iIntros "F"; iMod (INV0 with "F") as "[? _]"; iFrame. }
-      rewrite /IstProd in INV1. uPred.unseal_in INV1; destruct INV1 as [st_srcL [st_tgtL [st_srcR [st_tgtR INV1]]]].
-      destruct INV1 as [a1' [a1'' [INV1 [INV1' INV1'']]]]; inv INV1'.
-      rewrite /IstSB in INV1''; rr in INV1''; uPred.unseal_in INV1''; des.
-      destruct INV1''0 as [x0' [x0'' [? [INV1''0 ?]]]]; inv INV1''0.
-      destruct INV1''1 as [x1' [x1'' [? [INV1''1 ?]]]]; inv INV1''1.
-      rewrite /IstEq in H7; uPred.unseal_in H7; inv H7.
-      (*
-        new states after call should maintain the scope of previous states.
-        ctx state should maintain its own scope.
-      *)
-      eapply K; try refl; eauto using inv_sandbox_event; try nia; cycle 3.
-      { eapply nodup_app_l. rewrite <- map_app. eauto. }
-      { eapply nodup_app_l. rewrite <- map_app. eauto. }
-      iIntros "H". iPoseProof (INV0 with "H") as ">H".
-      iDestruct "H" as "[H1 H2]"; iModIntro; iSplitL "H1".
-      { rewrite INV1 INV1'' H2; iDestruct "H1" as "[_ [[_ H] _]]";
-          iPoseProof (Own_general_completeness with "H") as "H"; eauto. }
-      { iApply INV2; done. }
-    - mstep. i. eapply K; try refl; eauto using inv_sandbox_core.
-    - mstep. { rewrite alist_find_app_o. rewrite FUN. eauto. }
-      eapply K; try refl; eauto. grind.
-      rewrite! SBRed.bind.
-      move FLS at bottom. move FUN at bottom.
-      rewrite FLS in FUN.
-      rewrite alist_find_map_snd in FUN.
-      unfold o_map in FUN. des_ifs. unfold SB.sandbox_body.
-      destruct f0 as [[[img0 msk0] scp0] bd0]. s.
-      rewrite sandbox_well_scoped; eauto; cycle 1.
-      f_equal. extensionalities.
-      rewrite ?SBRed.bind !SBRed.tau SBRed.ret.
-      do 4 f_equal. extensionalities. eapply inv_sandbox_event; eauto.
-    - mstep. { rewrite alist_find_app_o. rewrite FUN. eauto. }
-      eapply K; try refl; eauto. grind.
-      rewrite! SBRed.bind.
-      move FLT at bottom. move FUN at bottom.
-      rewrite FLT in FUN.
-      rewrite alist_find_map_snd in FUN.
-      unfold o_map in FUN. des_ifs. unfold SB.sandbox_body.
-      destruct f0 as [[[img0 msk0] scp0] bd0]. s.
-      rewrite sandbox_well_scoped; eauto.
-      f_equal. extensionalities.
-      rewrite ?SBRed.bind !SBRed.tau SBRed.ret.
-      do 4 f_equal. extensionalities. eapply inv_sandbox_event; eauto.
-    - mstep. eapply K; try refl; eauto using inv_sandbox_tau.
-    - mstep. eapply K; try refl; eauto using inv_sandbox_tau.
-    - mstep. i. eapply K; try refl; eauto using inv_sandbox_core.
-    - mstep. i. eapply K; try refl; eauto using inv_sandbox_core.
-    - mstep. eapply K; try refl; eauto using inv_sandbox_core.
-    - mstep. eapply K; try refl; eauto using inv_sandbox_core.
-
-    - assert (H1:= ITRS).
-      rewrite  -ITRS SBRed.bind SBRed.put. des_ifs.
-      + mstep.
-        assert (UPD : alist_upd k v (st_src ++ st_ctx) = alist_upd k v st_src ++ st_ctx).
-        {
-          move SCPS at bottom. move SCPC at bottom.
-          eapply existsb_exists in Heq. des. eapply String.eqb_eq in Heq0.
-          rewrite alist_upd_not_tail; eauto.
-          ii. eapply NoDup_app_disjoint; eauto.
-          eapply in_map with (f:=fst) in H2.
-          rewrite List.map_map in H2. eapply SCPC in H2.
-          rewrite <- Heq0. eauto.
-        }
-        rewrite UPD. eapply K; try refl; eauto.
-        { rewrite state_scopes_update. eauto. }
-        { eapply sandbox_well_scoped; et; refl. }
-        { f_equal. symmetry. eapply inv_sandbox_pg. eauto. }
-      + unfold triggerUB. ired. mstep. ss.
-
-  - assert (H1:=ITRT).
-    rewrite -ITRT SBRed.bind SBRed.put. des_ifs.
-    + mstep.
-      assert (UPD : alist_upd k v (st_tgt ++ st_ctx) = alist_upd k v st_tgt ++ st_ctx).
-      {
-        move SCPS at bottom. move SCPC at bottom.
-        eapply existsb_exists in Heq. des. eapply String.eqb_eq in Heq0.
-        eapply alist_upd_not_tail. eauto.
-        ii. eapply NoDup_app_disjoint; eauto.
-        eapply in_map with (f:=fst) in H2.
-        rewrite List.map_map in H2. eapply SCPC in H2.
-        rewrite <- Heq0. eauto.
-      }
-      rewrite UPD. eapply K; try refl; eauto.
-      { rewrite state_scopes_update. eauto. }
-      { eapply sandbox_well_scoped; et. refl. }
-      { f_equal. symmetry. eapply inv_sandbox_pg. eauto. }
-    + rewrite SBRed.bind SBRed.put Heq !bind_trigger in H1.
-      exfalso. unfold triggerUB in H1. rewrite bind_bind bind_vis in H1. ss.
-
-  - assert (H1:=ITRS).
-    rewrite  -ITRS SBRed.bind SBRed.get. des_ifs.
-    + mstep. eapply K; try refl; eauto.
-      { eapply sandbox_well_scoped; et. refl. }
-      erewrite alist_find_exists_l; eauto.
-      repeat f_equal. symmetry. eapply inv_sandbox_pg; eauto.
-    + unfold triggerUB. ired. mstep. ss.
-
-  - assert (H1:=ITRT).
-    rewrite  -ITRT SBRed.bind SBRed.get. des_ifs.
-    + mstep. eapply K; try refl; eauto.
-      { eapply sandbox_well_scoped; et. refl. }
-      erewrite alist_find_exists_l; eauto.
-      repeat f_equal. symmetry. eapply inv_sandbox_pg; eauto.
-    + rewrite SBRed.bind SBRed.get Heq !bind_trigger in H1.
-      exfalso. unfold triggerUB in H1. rewrite bind_bind bind_vis in H1. ss.
-
-  - mstep. i. eapply K; try refl; eauto using inv_sandbox_ag.
-  - mstep. i. eapply K; try refl; eauto using inv_sandbox_ag.
-  - mstep. i. eapply K; try refl; eauto using inv_sandbox_ag.
-  - mstep. i. eapply K; try refl; eauto using inv_sandbox_ag.
-  - mstep. i. eapply K; try refl; eauto using inv_sandbox_ag.
-  - mstep. i. eapply (K fmr1); et; i; des.
-    try refl; eauto using inv_sandbox_ag.
-  (* - guclo @msimC_spec. econs; esplits; et.
-    eapply msim_assume_res_both; et.
-    i. eapply K; try refl; eauto using inv_sandbox_ag. *)
-  - mstep. intros tid; eapply (K tid); try refl; eauto.
-    + eapply inv_sandbox_spawn in ITRT. eauto.
-    + eapply inv_sandbox_spawn in ITRS. eauto.
-  - mstep.
-    { instantiate (1:= FR). iIntros "H". iPoseProof (INV with "H") as ">[H FR]".
-      iModIntro. iFrame. iExists st_ctx, st_ctx.
-      iSplit; eauto.
-    }
-    i. guclo msim_wfC_spec. econs. i.
-    eapply Own_bupd_split in INV0; eauto. des.
-    eapply Own_general_soundness in INV1; eauto; cycle 1.
-    { by eapply Own_wand_valid; first by iIntros "F"; iMod (INV0 with "F") as "[? _]"; iFrame. }
-    rewrite /IstProd in INV1. uPred.unseal_in INV1; destruct INV1 as [st_srcL [st_tgtL [st_srcR [st_tgtR INV1]]]].
-    destruct INV1 as [a1' [a1'' [INV1 [INV1' INV1'']]]]; inv INV1'.
-    rewrite /IstSB in INV1''; rr in INV1''; uPred.unseal_in INV1''; des.
-    destruct INV1''0 as [x0' [x0'' [? [INV1''0 ?]]]]; inv INV1''0.
-    destruct INV1''1 as [x1' [x1'' [? [INV1''1 ?]]]]; inv INV1''1.
-    rewrite /IstEq in H7; uPred.unseal_in H7; inv H7.
-    (*
-      new states after call should maintain the scope of previous states.
-      ctx state should maintain its own scope.
-    *)
-    eapply K; try refl; eauto; try nia; cycle 3.
-    { rewrite SBRed.bind SBRed.yield !bind_trigger in ITRT.
-      depdes ITRT. eapply equal_f in x. eauto. }
-    { rewrite SBRed.bind SBRed.yield !bind_trigger in ITRS.
-      depdes ITRS. eapply equal_f in x. eauto. }
-    { eapply nodup_app_l. rewrite <- map_app. eauto. }
-    { eapply nodup_app_l. rewrite <- map_app. eauto. }
-    iIntros "H". iPoseProof (INV0 with "H") as ">H".
-    iDestruct "H" as "[H1 H2]"; iModIntro; iSplitL "H1".
-    { rewrite INV1 INV1'' H2; iDestruct "H1" as "[_ [[_ H] _]]";
-        iPoseProof (Own_general_completeness with "H") as "H"; eauto. }
-    { iApply INV2; done. }
-
-  - mstep. intros tid; eapply (K tid); try refl; eauto.
-    + eapply inv_sandbox_gettid in ITRT. eauto.
-    + eapply inv_sandbox_gettid in ITRS. eauto.
-
-  - gstep. econs. econs. econs; eauto. econs; eauto.
-    gbase. pclearbot. eapply CIH; try refl; eauto. *)
-Admitted.
-
-Lemma isim_ctx `{Σ : GRA} contextual RR fs ft ms mt ctx Ist :
-  (* (WFS : Mod.wf (ms ★ ctx))
-  (WFT : Mod.wf (mt ★ ctx))
-  (SCOPES : sub_perm (Mod.scopes ms) (Mod.scopes mt))
-  (NODUPFT : List.NoDup (List.map fst (Mod.fnsems mt ++ Mod.fnsems ctx)))
-  (NODUPFS : List.NoDup (List.map fst (Mod.fnsems ms ++ Mod.fnsems ctx))) *)
-  ∀ (arg : Any.t) st_src st_tgt st_ctx,
-    (elements (dom st_src)).*1 ⊆ Mod.scopes mt →
-    (elements (dom st_tgt)).*1 ⊆ Mod.scopes mt →
-    Mod.scopes ms ⊆+ Mod.scopes mt →
-    Mod.wf (ms ★ ctx) →
-    Mod.wf (mt ★ ctx) →
-    (* (SCOPEFS: incl fs.1.2 (Mod.scopes mt))
-    (SCOPEFT: incl ft.1.2 (Mod.scopes mt))
-    (SCOPES: incl (map (fst∘fst) st_src) (Mod.scopes mt))
-    (SCOPET: incl (map (fst∘fst) st_tgt) (Mod.scopes mt))
-    (SCOPEC: incl (map (fst∘fst) st_ctx) (Mod.scopes ctx)),
-     *)
-    isim open
-      ((λ v : option _, SB.sandbox_body <$> v) <$> (Mod.fnsems ms))
-      ((λ v : option _, SB.sandbox_body <$> v) <$> (Mod.fnsems mt))
-      Ist ibot ibot (ist_with_eq RR) false false
-      (st_src, SB.sandbox_body fs arg)
-      (st_tgt, SB.sandbox_body ft arg) ⊢
-    @isim _ contextual
-      ((λ v : option _, SB.sandbox_body <$> v) <$> (Mod.fnsems (ms ★ ctx)))
-      ((λ v : option _, SB.sandbox_body <$> v) <$> (Mod.fnsems (mt ★ ctx)))
-      (IstProd (IstSB (Mod.scopes mt) Ist) IstEq)
-      ibot ibot Any.t Any.t
-      (ist_with_eq (IstProd (IstSB (Mod.scopes mt) RR) IstEq))
-      false false
-      (union_with (const (const (Some None))) st_src st_ctx, SB.sandbox_body fs arg)
-      (union_with (const (const (Some None))) st_tgt st_ctx, SB.sandbox_body ft arg).
+Lemma isim_ctx `{Σ : GRA} contextual RR fs ft ms mt ctx Ist arg st_src st_tgt st_ctx :
+  (elements (dom st_src)).*1 ⊆ Mod.scopes mt →
+  (elements (dom st_tgt)).*1 ⊆ Mod.scopes mt →
+  (elements (dom st_ctx)).*1 ⊆ Mod.scopes ctx →
+  Mod.scopes ms ⊆+ Mod.scopes mt →
+  Mod.wf (ms ★ ctx) →
+  Mod.wf (mt ★ ctx) →
+  (∃ fno, Mod.fnsems ms !! fno = Some (Some fs) ∧ Mod.fnsems mt !! fno = Some (Some ft)) →
+  isim open
+    ((λ v : option _, SB.sandbox_body <$> v) <$> (Mod.fnsems ms))
+    ((λ v : option _, SB.sandbox_body <$> v) <$> (Mod.fnsems mt))
+    Ist ibot ibot (ist_with_eq RR) false false
+    (st_src, SB.sandbox_body fs arg)
+    (st_tgt, SB.sandbox_body ft arg) ⊢
+  @isim _ contextual
+    ((λ v : option _, SB.sandbox_body <$> v) <$> (Mod.fnsems (ms ★ ctx)))
+    ((λ v : option _, SB.sandbox_body <$> v) <$> (Mod.fnsems (mt ★ ctx)))
+    (IstProd (IstSB (Mod.scopes mt) Ist) (IstSB (Mod.scopes ctx) IstEq))
+    ibot ibot Any.t Any.t
+    (ist_with_eq (IstProd (IstSB (Mod.scopes mt) RR) (IstSB (Mod.scopes ctx) IstEq)))
+    false false
+    (union_with (const (const (Some None))) st_src st_ctx, SB.sandbox_body fs arg)
+    (union_with (const (const (Some None))) st_tgt st_ctx, SB.sandbox_body ft arg).
 Proof.
-  intros arg st_src st_tgt st_ctx Hsrc Htgt Hscp Hwfs Hwft; apply entails_pointwise => r Hsim.
+  intros Hsrc Htgt Hctx Hscp Hwfs Hwft Hin.
+  apply entails_pointwise => r Hsim.
   eapply isim_init in Hsim; eauto.
   eapply gpaco8_mon in Hsim; try apply iunlift_ibot.
   eapply gpaco8_init in Hsim; eauto with paco.
@@ -850,87 +267,37 @@ Proof.
   eapply paco8_mon_bot; eauto.
   destruct fs as [msks bds]; destruct ft as [mskt bdt].
   eapply msim_ctx; eauto.
-  { rewrite /SB.sandbox_body /=. admit.
+  { destruct Hin as [fno [Hins Hint]].
+    eapply sandbox_well_scoped; ss.
+    intros ? s; depdes s; ss; depdes s; ss; depdes s; ss.
+    depdes p; ss; hexploit (Mod.well_scoped_fns ms); rewrite map_Forall_lookup =>
+      /(_ fno (msks, bds)); rewrite lookup_omap Hins => /(_ eq_refl);
+      [intros [Hkey ?]|intros [? Hkey]] => /Hkey; case_decide; ss;
+      intros Hin; eapply elem_of_submseteq in Hin; eauto.
   }
-  { admit. }
-Admitted.
-  (* etrans; eauto.
-  apply submseteq_Permutation in Hscp as [? ->]; set_solver.  *)
-(* Qed. *)
-  (* ii. rewrite /SB.sandbox_body.
-  eapply entails_pointwise. intros fmr SIM.
-  eapply isim_init in SIM; cycle 1; et.
-  eapply gpaco8_mon in SIM; try apply iunlift_ibot.
-  eapply gpaco8_init in SIM; eauto with paco.
-  eapply isim_final, gpaco8_final; eauto with paco. right.
-  eapply paco8_mon_bot; et.
-  destruct fs as [[[img msk] scp] bd].
-  destruct ft as [[[img0 msk0] scp0] bd0]. ss.
-  rewrite !map_app. eapply msim_ctx; try apply SIM; try nia; cycle 8; i.
-  - instantiate (1:= wmask_all). instantiate (1:= true).
-    rewrite sandbox_well_scoped; i; bsimpl; et.
-  - rewrite sandbox_well_scoped; i; bsimpl; et.
-  - refl.
-  - refl.
-  - bsimpl. esplits; et.
-    etrans; [|eapply sub_perm_incl; et].
-    etrans; [|eapply Mod.well_scoped_fns].
-    unfold fnsems_scopes. erewrite IN. refl.
-  - bsimpl. esplits; et.
-    etrans; [|eapply Mod.well_scoped_fns].
-    unfold fnsems_scopes. erewrite IN. refl.
-  - destruct WFT. et.
-  - et.
-  - etrans; [apply SCOPES0|]. refl.
-  - et.
-Qed. *)
+  { destruct Hin as [fno [Hins Hint]].
+    eapply sandbox_well_scoped; ss.
+    intros ? s; depdes s; ss; depdes s; ss; depdes s; ss.
+    depdes p; ss; hexploit (Mod.well_scoped_fns mt); rewrite map_Forall_lookup =>
+      /(_ fno (mskt, bdt)); rewrite lookup_omap Hint => /(_ eq_refl);
+      [intros [Hkey ?]|intros [? Hkey]] => /Hkey; case_decide; ss;
+      intros Hin; eapply elem_of_submseteq in Hin; eauto.
+  }
+Qed.
 
 Section ADEQUACY.
   Context `{!crisG Γ Σ α β τ _S _I}.
 
   Lemma ISim_ctx contextual (ms mt ctx : Mod.t) IC Ist : 
     ISim.t open ms mt IC Ist →
-    ISim.t contextual (ms ★ ctx) (mt ★ ctx) IC (IstProd (IstSB mt.(Mod.scopes) Ist) IstEq).
+    ISim.t contextual (ms ★ ctx) (mt ★ ctx) IC
+      (IstProd (IstSB mt.(Mod.scopes) Ist) (IstSB ctx.(Mod.scopes) IstEq)).
   Proof using.
     intros Hsim; apply ISim.t_strong; intros Hwftctx.
     hexploit Mod.add_wf; eauto; intros [Hwft Hwfctx].
     hexploit ISim_wf; eauto; intros Hwfs.
     pose Hsim as Hsim'; destruct Hsim' as [Hscp Hic Hsimfun].
-    eapply ISim_reflR; eauto.
-    { intros fn Hfns; hexploit ISim_match; eauto; intros [fbot Hfnt]%elem_of_dom.
-      apply elem_of_dom in Hfns as [fbos Hfns].
-      assert (Hfnctx : Mod.fnsems ctx !! fn = None).
-      { destruct (_ ctx !! fn) eqn : Hctx; ss.
-        exfalso; hexploit Mod.wf_fns; [apply Hwftctx|].
-        rewrite map_Forall_lookup /= => /(_ fn None); rewrite lookup_union_with Hfnt Hctx //=.
-        intros []; ss.
-      }
-      rewrite /ISim.sim_fun /= ?lookup_fmap ?lookup_union_with Hfnctx Hfns Hfnt /=.
-      destruct fbos as [fbs|]; ss; cycle 1.
-      { hexploit (Hsimfun Hwft fn); rewrite /ISim.sim_fun lookup_fmap Hfns /= Hfnt //. }
-      destruct fbot as [fbt|]; ss; cycle 1.
-      { hexploit (Hsimfun Hwft fn); rewrite /ISim.sim_fun ?lookup_fmap Hfns Hfnt /=.
-        intros Hf; hexploit Hf; eauto; i; des; clarify.
-      }
-      intros _ _; eexists; split; first refl.
-      intros arg st_src st_tgt.
-      iIntros "[% [% [% [%st_ctx [[-> ->] [[[% %] IST] ->]]]]]] WINV".
-      iApply isim_ctx; eauto. { admit. }
-      hexploit (Hsimfun Hwft fn); rewrite /ISim.sim_fun ?lookup_fmap Hfns Hfnt /= => /(_ Hwfs Hwft).
-      intros [? [? Hisim]]; clarify; move : Hisim => /(_ arg st_srcL st_tgtL); intros Hisim.
-      iApply (Hisim with "IST WINV").
-    }
-    { intros ? ?; eapply ISim_match; eauto. }
-    { rewrite Hic //; iIntros "$"; iExists _, _; iSplit; eauto.
-      iSplit; eauto.
-      iPureIntro; split; [|destruct mt; ss].
-      etrans; first apply (Mod.well_scoped_init).
-      hexploit Hscp; eauto; clear Hscp; intros Hscp.
-      apply submseteq_Permutation in Hscp as [? ->]; set_solver.
-    }
-Admitted.
-Search Mod.t ISim.t Mod.wf.
-    (* econs; intros [Hwft Hwfctx]%Mod.add_wf.
+    econs; intros _.
     { apply submseteq_app; eauto. }
     { rewrite Hic //; iIntros "$"; iExists _, _; iSplit; eauto.
       iSplit; eauto.
@@ -941,118 +308,47 @@ Search Mod.t ISim.t Mod.wf.
       }
       iSplit; [iPureIntro; split; destruct ctx; ss|ss].
     }
-    hexploit ISim_wf; eauto; intros Hwfs.
-    intros fn; rewrite /ISim.sim_fun ?lookup_fmap /= ?lookup_union_with.
-    destruct (_ ms !! fn) as [[[mskms itrms]|]|] eqn : Hms; cycle 1.
-    { inv Hwfs; rewrite map_Forall_lookup in wf_fns; hexploit (wf_fns _ _ Hms).
-      intros []; clarify.
+    intros fno; move: Hsimfun => /(_ Hwft fno).
+    rewrite /ISim.sim_fun ?lookup_fmap /= ?lookup_union_with.
+    destruct (_ ms !! fno) as [[[fmsk fbd]|]|] eqn: Hfnoms; ss.
+    { move => /= /(_ Hwfs Hwft) [? [? Hsimfun]].
+      destruct (_ mt !! fno) as [[[fmskt fbdt]|]|] eqn : Hfnomt; ss; clarify.
+      destruct (_ ctx !! fno) as [|]; ss; intros ??; esplits; eauto.
+      iIntros (arg st_src st_tgt) "[% [% [% [% [[-> ->] [[[% %] IST] [[% _] ->]]]]]]] W".
+      iApply isim_ctx; eauto.
+      iApply (Hsimfun arg _ _ with "IST W").
     }
-    { destruct (_ ctx !! fn) as [[[mskctx itrctx]|]|] eqn : Hctx; ss.
-      { intros _ Hwf; destruct (_ mt !! fn) eqn : Hmt; ss.
-        { exfalso; hexploit (Mod.wf_fns _ Hwf); rewrite map_Forall_lookup.
-          intros Hf; hexploit (Hf fn None); [|intros []; clarify].
-          rewrite /= lookup_union_with Hctx Hmt //=.
+    { exfalso; move: (Mod.wf_fns ms Hwfs).
+      rewrite map_Forall_lookup => /(_ fno None Hfnoms) [??] //.
+    }
+    { destruct (_ ctx !! fno) as [[[fmsk fbd]|]|] eqn : Hfnoctx; ss.
+      { intros _ ? ?.
+        destruct (_ mt !! fno) eqn : Hmt; ss.
+        { exfalso; move: (Mod.wf_fns _ Hwftctx); rewrite map_Forall_lookup => /(_ fno None) /=.
+          rewrite lookup_union_with Hmt Hfnoctx //= => /(_ eq_refl) => [[??]] //.
         }
-        eexists; split; first done.
-        eapply 
+        eexists; split; [done|].
+        apply isim_reflR; eauto.
+        { intros ???? Hkey; hexploit (Mod.well_scoped_fns ctx fno (fmsk, fbd)).
+          { rewrite lookup_omap Hfnoctx //. }
+          intros [Hmsk _]; move: Hmsk => /(_ k v Hkey) ?; split.
+          { iIntros "[% ->]"; iSplit; [rewrite ?dom_insert_L|eauto]; iPureIntro.
+            split; set_solver.
+          }
+          hexploit (Mod.wf_scopes _ Hwftctx) => /NoDup_app [? [? _]]; set_solver.
+        }
+        { intros ??? Hkey; hexploit (Mod.well_scoped_fns ctx fno (fmsk, fbd)).
+          { rewrite lookup_omap Hfnoctx //. }
+          intros [_ Hmsk]; move: Hmsk => /(_ k Hkey) ?; split.
+          { iIntros "[% ->] //". }
+          hexploit (Mod.wf_scopes _ Hwftctx) => /NoDup_app [? [? _]]; set_solver.
+        }
       }
-      2:{ }
-    }
-    destruct (_ ctx !! fn) eqn : Hctx; ss.
-    { hexploit (Hsimfun Hwft fn); rewrite /ISim.sim_fun ?lookup_fmap Hms /=.
-
-      des_ifs; ss 2:{ }
-    }
-
-    i. hexploit (sim_fnsems WFT fn); et. intros SIM.
-    destruct fn; cycle 1.
-    { ii. ss. rewrite !alist_find_app_o in FIND |- *.
-      destruct (alist_find _ (Mod.fnsems ms)) eqn: E0; inv FIND.
-      - exploit SIM; et.
-        { rewrite map_app in NODUPFS. eapply NoDup_app_remove_r; et. }
-        { rewrite map_app in NODUPFT. eapply NoDup_app_remove_r; et. }
-        i; des. rewrite x0. esplits; et.
-        ii. destruct fs as [[[img msk] scp] bd].
-        destruct ft as [[[img0 msk0] scp0] bd0].
-        iIntros "[% H] I". des; subst.
-        iApply isim_mono; cycle 1.
-        { iApply isim_ctx; et; try apply Mod.well_scoped_init.
-          - s. etrans; cycle 1.
-            { eapply sub_perm_incl. et. }
-            etrans; [|eapply Mod.well_scoped_fns].
-            rewrite /fnsems_scopes. erewrite E0. refl.
-          - s. etrans; [|eapply Mod.well_scoped_fns].
-            rewrite /fnsems_scopes. erewrite x0. refl.
-          - etrans; [eapply Mod.well_scoped_init|].
-            eapply sub_perm_incl; et.
-          - exploit x1; et. i.
-            iApply (x2 with "[H]"); et. iSplit; et.
-        }
-        i. iIntros "%". des; subst. iPureIntro. et.
-
-      - destruct (alist_find None (Mod.fnsems mt)) eqn: E.
-        { exfalso. rewrite map_app in NODUPFT.
-          eapply NoDup_app_disjoint; eauto.
-          - eapply alist_find_some, (in_map fst) in E. et.
-          - eapply alist_find_some, (in_map fst) in H0. et.
-        }
-        rewrite H0. esplits; et. ii.
-        destruct fs as [[[img msk] scp] bd].
-        iIntros "[% H] I". des; subst.
-        iApply isim_mono; cycle 1.
-        { iApply (isim_reflR with "[H]"); et.
-          - eapply WFT0.
-          - s. etrans; [|eapply Mod.well_scoped_fns].
-            rewrite /fnsems_scopes. erewrite H0. refl.
-          - i. iIntros "%". des; subst. et.
-          - i. iIntros "%". des; subst. iPureIntro.
-            rewrite state_scopes_update. et.
-          - exploit sim_initial; et; try rewrite !alist_find_map_snd.
-            { rewrite E. et. }
-            i. des. rewrite x1. do 4 iExists _. iSplit; et.
-            rewrite /IstSB. iSplit.
-            + iFrame. iPureIntro. split; try apply Mod.well_scoped_init.
-              etrans; try apply Mod.well_scoped_init.
-              eapply sub_perm_incl. et.
-            + iSplit; et. iPureIntro. split; apply Mod.well_scoped_init.
-        }
-        i. iIntros "[% H]". subst. iPureIntro. et.
-    }
-
-    ii. ss. rewrite alist_find_app_o in FIND. des_ifs.
-    {
-      (* find in src/tgt module *)
-      exploit sim_fnsems; et; try eapply WFS; try eapply WFT. i; des.
-      esplits.
-      { rewrite alist_find_app_o. des_ifs. }
-      ii. iIntros "[% [% [% [% [% [[% H] %]]]]]] I". des; subst.
-      iApply (isim_ctx with "[H I]"); et; i.
-      - etrans; [|eapply sub_perm_incl; et].
-        etrans; [|eapply Mod.well_scoped_fns].
-        unfold fnsems_scopes. erewrite Heq. destruct fs, p. refl.
-      - etrans; [|eapply Mod.well_scoped_fns].
-        unfold fnsems_scopes. erewrite x0. destruct ft, p. refl.
-      - exploit x1; cycle 2; i.
-        + iApply (x2 with "[H]"); et.
-    }
-    {
-      exists fs. esplits; ss.
-      { rewrite alist_find_app_o. des_ifs. exfalso.
-        eapply alist_find_some in FIND, Heq0.
-        eapply in_map with (f:=fst) in FIND, Heq0.
-        rewrite map_app in NODUPFT.
-        eapply NoDup_app_disjoint; eauto.
+      { exfalso; move: (Mod.wf_fns ctx Hwfctx).
+        rewrite map_Forall_lookup => /(_ fno None Hfnoctx) [??] //.
       }
-      destruct fs as [[[img msk] sc] bd].
-      inv WFTC. eapply isim_reflR; ss; i; eauto.
-      - etrans; [|eapply Mod.well_scoped_fns].
-        rewrite /fnsems_scopes. erewrite FIND. refl.
-      - iIntros "%". des; subst; eauto.
-      - iIntros "%". des; subst; eauto. iPureIntro.  esplits; eauto.
-        + rewrite state_scopes_update. eauto.
-        + rewrite state_scopes_update. eauto.
     }
-  Qed. *)
+  Qed.
 
   Theorem main_adequacy (ms mt : Mod.t) IC Ist :
     ISim.t open ms mt IC Ist →
